@prefix rdf: <http://www.w3.org/1999/02/22-rdf-syntax-ns#> .
@prefix rdfs: <http://www.w3.org/2000/01/rdf-schema#> .
@prefix owl: <http://www.w3.org/2002/07/owl#> .
@prefix xsd: <http://www.w3.org/2001/XMLSchema#> .
@prefix dct: <http://purl.org/dc/terms/> .
@prefix skos: <http://www.w3.org/2004/02/skos/core#> .
@prefix cc: <http://creativecommons.org/ns#> .
@prefix era: <http://data.europa.eu/949/> .
@prefix era-skos: <http://data.europa.eu/949/concepts/> .

@prefix era-trd: <http://data.europa.eu/949/concepts/track-running-directions/> .
@prefix era-trd-rinf: <http://data.europa.eu/949/concepts/track-running-directions/rinf/> .


#################################################################
#
#    Concept Schemes
#
#################################################################



era-trd:TrackRunningDirections a skos:ConceptScheme ;
    dct:issued "2020-09-01"^^xsd:date ;
    dct:modified "2022-09-09"^^xsd:date ;
    cc:license <https://creativecommons.org/licenses/by/4.0/> ;
    rdfs:comment "Controlled SKOS-based vocabularies defined by the European Union Agency for Railways to describe concepts related to the European railway infrastructure and the vehicles authorized to operate over it."@en ;
    rdfs:label "Track Running Directions"@en ;
    skos:prefLabel "Track Running Directions"@en ;
    dct:title "Concept scheme grouping track running directions"@en .

#################################################################
#
#    Concept instances
#
#################################################################


########## Track running directions ##########

era-trd-rinf:10 a skos:Concept;
  skos:inScheme era-trd:TrackRunningDirections; skos:topConceptOf era-trd:TrackRunningDirections;
  skos:prefLabel "N" ; skos:note "Value retrieved from the RINF database";
  skos:definition "The normal runnig direction is the same as the direction defined by the start and end of the Section of Line." .

era-trd-rinf:20 a skos:Concept;
  skos:inScheme era-trd:TrackRunningDirections; skos:topConceptOf era-trd:TrackRunningDirections;
  skos:prefLabel "O" ; skos:note "Value retrieved from the RINF database";
  skos:definition "The normal runnig direction is the opposite as the direction defined by the start and end of the Section of Line." .

era-trd-rinf:30 a skos:Concept;
  skos:inScheme era-trd:TrackRunningDirections; skos:topConceptOf era-trd:TrackRunningDirections;
  skos:prefLabel "B" ; skos:note "Value retrieved from the RINF database";
  skos:definition "The normal runnig direction is both directions defined by the Section of Line." .
